\documentclass[12pt]{article}
\usepackage{paralist,amsmath,amssymb,thumbpdf,lmodern}
\usepackage{algorithm}
\usepackage{algpseudocode}
\usepackage[margin=0.5in]{geometry}
\usepackage{graphicx}
\usepackage{enumerate}
\usepackage{physics}
\usepackage{amsfonts}
\usepackage{bbm}
\usepackage{xcolor}
\usepackage{subcaption}
\usepackage{graphicx}
\usepackage{multirow}
\usepackage{amsfonts}
\usepackage{booktabs}
\usepackage{diagbox}
\usepackage[outdir=./]{epstopdf}
\usepackage{caption}
\usepackage{bm}
\usepackage{makecell}
\usepackage{ifxetex,ifluatex}
\newcommand*\diff{\mathop{}\!\mathrm{d}}
\begingroup\expandafter\expandafter\expandafter\endgroup
\expandafter\ifx\csname IncludeInRelease\endcsname\relax
  \usepackage{fixltx2e}
\fi
\ifnum 0\ifxetex 1\fi\ifluatex 1\fi=0 % if pdftex
  \usepackage[T1]{fontenc}
  \usepackage[utf8]{inputenc}
  \usepackage{textcomp} % provides euro and other symbols
\else % if luatex or xelatex
  \usepackage{unicode-math}
  \defaultfontfeatures{Ligatures=TeX,Scale=MatchLowercase}
\fi
\usepackage{hyperref}
\hypersetup{
    colorlinks=true,
    linkcolor=blue,
    filecolor=magenta,      
    urlcolor=blue,
}
\urlstyle{same}  % don't use monospace font for urls
\setlength{\emergencystretch}{3em}  % prevent overfull lines
\usepackage{newtxtext,newtxmath}

\title{Biostat 830 HW3}
\date{}
\author{Mukai Wang 98830336}

\makeatletter
\newenvironment{breakablealgorithm}
{% \begin{breakablealgorithm}
		\begin{center}
			\refstepcounter{algorithm}% New algorithm
			\hrule height.8pt depth0pt \kern2pt% \@fs@pre for \@fs@ruled
			\renewcommand{\caption}[2][\relax]{% Make a new \caption
				{\raggedright\textbf{\fname@algorithm~\thealgorithm} ##2\par}%
				\ifx\relax##1\relax % #1 is \relax
				\addcontentsline{loa}{algorithm}{\protect\numberline{\thealgorithm}##2}%
				\else % #1 is not \relax
				\addcontentsline{loa}{algorithm}{\protect\numberline{\thealgorithm}##1}%
				\fi
				\kern2pt\hrule\kern2pt
			}
		}{% \end{breakablealgorithm}
		\kern2pt\hrule\relax% \@fs@post for \@fs@ruled
	\end{center}
}
\makeatother


\begin{document}
\maketitle

\section*{Problem 1}

\begin{enumerate}[(a)]

\item  The Poisson Gamma process sets up the observed counts $Y_t$ and hidden state $\theta_t$, $\left.Y_t\right\vert\theta_t \sim \text{Poisson}(a_t \theta_t)$. For all time points $t=0,1,2,\cdots, T$, marginally $\theta_t \sim \text{Gamma}(\lambda, 1/\lambda)$ which means $E[\theta_t] = 1$, $\text{Var}(\theta_t)=1/\lambda$. The $\{\theta_t \}_{t=1,2,\cdots T}$ follows an AR(1) model $\theta_t = B_t \theta_{t-1}+\varepsilon_t$. $B_t \stackrel{iid}{\sim} \text{Beta}(\rho\lambda, (1-\rho)\lambda)$ and $\varepsilon_{t} \stackrel{iid}{\sim} \text{Gamma}((1-\rho)\lambda, 1/\lambda)$. Therefore $E[B_t] = \rho$ and $\text{Var}(B_t) = \frac{\rho (1-\rho)}{\lambda + 1}$. $\mathbb{E}[\varepsilon_t] = 1-\rho$ and $\text{Var}(\varepsilon_t) = \frac{1 - \rho}{\lambda}$.

During forward Kalman filtering, suppose we have got the BLUE (best linear unbiased estimator) of $\theta_{t-1}$ and its expected squared prediction error, $\left. \theta_{t-1} \right\vert Y^{t-1} \sim [m_{t-1}; c_{t-1}]$. Then we can derive the BLUE of $\left. \theta_{t} \right\vert Y^{t-1}$ and $\left. Y_{t} \right\vert Y^{t-1}$ as well as their expected squared prediction errors.
\begin{align}
	 E\left[\left. \theta_t \right\vert Y^{t-1}\right]&=E\left[ \left.E[\left. \theta_{t} \right\vert \theta_{t-1}]\right\vert Y^{t-1} \right] \nonumber \\ 
	&= E\left[\left. \rho\theta_{t-1}+1-\rho\right\vert Y^{t-1} \right] \nonumber\\ 
	&=\rho m_{t-1} + 1 - \rho 	
\end{align}
\begin{align}
	H_t \stackrel{\text{def}}{=} \text{Var}\left(\left. \theta_t\right\vert Y^{t-1} \right) &= E\left[\left. \text{Var}\left(\left.\theta_t\right\vert \theta_{t-1} \right) \right\vert Y^{t-1} \right] + \text{Var}\left( \left.   E\left[\left. \theta_{t} \right\vert \theta_{t-1} \right]\right\vert Y^{t-1} \right) \nonumber \\
	&= E\left[ \left. \theta_{t-1}^2\cdot \frac{\rho(1-\rho)}{\lambda + 1} + \frac{1-\rho}{\lambda} \right\vert Y^{t-1} \right] +\text{Var}\left( \left. \rho \cdot \theta_{t-1}+1-\rho \right\vert Y^{t-1} \right) \nonumber \\
	&= \frac{1-\rho^2}{\lambda} + \rho^2 \cdot c_{t-1}
\end{align}
\begin{align}
	f_{t} \stackrel{\text{def}}{=} E\left[\left. Y_{t} \right\vert Y^{t-1} \right] &= E\left[ \left. E\left[ \left. Y_{t} \right\vert \theta_{t} \right] \right\vert Y^{t-1} \right] \nonumber \\
	&= a_{t}(\rho m_{t-1}+1-\rho)
\end{align}
\begin{align}
	Q_{t} \stackrel{\text{def}}{=} \text{Var}\left(\left.Y_{t}\right\vert Y^{t-1} \right)&= E\left[\text{Var}\left( \left.Y_{t}\right\vert \theta_t \right) \right] + \text{Var}\left(\left. E\left[ \left.Y_{t}\right\vert\theta_t \right] \right\vert Y^{t-1} \right)\nonumber \\
	& = a_{t} + a_{t}^2 \left( \frac{1-\rho^2}{\lambda}+\rho^2 c_{t-1} \right)
\end{align}


If I denote $u_{t} = H_{t+1} = \frac{1-\rho^2}{\lambda}+\rho^2 c_{t}$, then plug in the fact that $E[B_{t+1}] = \rho$ and $E[b_{t+1}] = \bar{\rho} \stackrel{\text{def}}{=} 1-\rho$, we have
\begin{align}
	c_{t} \stackrel{\text{def}}{=} \text{Var}\left(\left. \theta_{t} \right\vert Y^{t} \right) &= H_t - H_t^{\top} A_{t}^{\top} Q_{t}^{-1} A_{t} H_t \nonumber\\
	&= u_{t-1} - \frac{a_{t}^2 u_{t-1}^2}{a_{t} + a_{t}^2 u_{t-1}} \nonumber\\
	&=\frac{u_{t-1}}{1+a_{t}u_{t-1}}
\end{align}
\begin{align}
	m_{t} \stackrel{\text{def}}{=} E\left[ \left. \theta_{t} \right\vert Y^{t} \right] &= B_{t}m_{t-1}+b_{t}+H_{t}^{\top}A_{t}^{\top}Q_{t}^{-1}(Y_{t}-f_{t})\nonumber \\
	&= \rho m_{t-1} + \bar{\rho} + \frac{a_{t}u_{t-1}}{a_{t}+a_{t}^2 u_{t-1}} (Y_{t} - f_{t})\nonumber \\
	&= \rho m_{t-1} + \bar{\rho}  + c_{t}(Y_{t} - f_{t})
\end{align}

The Kalman smoother given in page 26 of lecture note 3 tells us that 
\begin{align}
	m_{t}^{*} &= m_{t} + c_{t}B_{t+1}^{\top} H_{t+1}^{-1}(m_{t+1}^{*} - B_{t+1}m_{t} - b_{t+1}) 
\end{align}
Replacing the value of $B_{t+1}$ and $H_{t+1}$, and we have
\begin{align}
	m_{t}^{*}= m_{t} + \frac{\rho c_{t}}{u_{t}}(m_{t+1}^{*} - B_{t+1}m_{t} - b_{t+1})
\end{align}
This is the result that question (a) asks about.

\item According to page 26 of lecture note 3, the mean square prediction error of Kalman smoother is
\begin{align}
	c_{t}^{*} = c_{t} - c_{t}B_{t+1}^{\top} H_{t+1}^{-1} B_{t+1} c_{t} + c_{t}B_{t+1}^{\top} H_{t+1}^{-1} c_{t+1}^{*} H_{t+1}^{-1} B_{t+1} c_{t}
\end{align}

Replacing $B_{t+1}$ with $\rho$ and $H_{t+1}$ with $u_{t}$, we have
\begin{align}
	c_{t}^{*} &= c_{t} - \frac{\rho^2}{u_{t}}c_{t}^2 + \left( \frac{\rho c_{t}}{u_{t}} \right)^2 c_{t+1}^{*}\nonumber \\
	&= c_{t}\cdot \frac{u_{t} - \rho^2 c_{t}}{u_{t}} + \left( \frac{\rho c_{t}}{u_{t}} \right)^2 c_{t+1}^{*}\nonumber \\
	&= c_{t}\cdot \frac{1-\rho^2}{\lambda u_{t}} + \left( \frac{\rho c_{t}}{u_{t}} \right)^2 c_{t+1}^{*}
\end{align}
This is the result that question (b) asks about.


\end{enumerate}



\section*{Problem 2}





\section*{Problem 3}


	




\end{document}
